fix compilation

erasure/theories/EEtaExpanded.v
@@ -1,3 +1,313 @@
+(* Distributed under the terms of the MIT license. *)
+From Coq Require Import Utf8 Program.
+From MetaCoq.Template Require Import config utils Kernames.
+From MetaCoq.PCUIC Require Import PCUICAst PCUICAstUtils
+     PCUICReflect PCUICWeakeningEnvConv PCUICWeakeningEnvTyp
+     PCUICTyping PCUICInversion PCUICGeneration
+     PCUICConfluence PCUICConversion 
+     PCUICCumulativity PCUICSR PCUICSafeLemmata
+     PCUICValidity PCUICPrincipality PCUICElimination PCUICSN.
+
+From MetaCoq.SafeChecker Require Import PCUICWfEnv.
+     
+From MetaCoq.Erasure Require Import EAst EAstUtils EInduction EArities Extract Prelim
+    ELiftSubst ESpineView ECSubst.
+
+Local Open Scope string_scope.
+Set Asymmetric Patterns.
+Import MCMonadNotation.
+
+From Equations Require Import Equations.
+Set Equations Transparent.
+Local Set Keyed Unification.
+From Coq Require Import ssreflect ssrbool.
+
+(** We assume [Prop </= Type] and universes are checked correctly in the following. *)
+Local Existing Instance extraction_checker_flags.
+
+Ltac introdep := let H := fresh in intros H; depelim H.
+
+#[global]
+Hint Constructors Ee.eval : core.
+
+Set Warnings "-notation-overridden".
+Import E.
+Set Warnings "+notation-overridden".
+
+
+Section AllInP.
+  Context {A : Type}.
+
+  Equations forallb_InP (l : list A) (H : forall x : A, In x l -> bool) : bool :=
+  | nil, _ := true ;
+  | (cons x xs), H := (H x _) && (forallb_InP xs (fun x inx => H x _)).
+End AllInP.
+
+Lemma forallb_InP_spec {A} (f : A -> bool) (l : list A) :
+  forallb_InP l (fun x _ => f x) = List.forallb f l.
+Proof.
+  remember (fun x _ => f x) as g.
+  funelim (forallb_InP l g) => //; simpl. f_equal.
+  now rewrite (H0 f).
+Qed.
+
+Section MapInP.
+  Context {A B : Type}.
+
+  Equations map_InP (l : list A) (f : forall x : A, In x l -> B) : list B :=
+  map_InP nil _ := nil;
+  map_InP (cons x xs) f := cons (f x _) (map_InP xs (fun x inx => f x _)).
+End MapInP.
+
+Lemma map_InP_spec {A B : Type} (f : A -> B) (l : list A) :
+  map_InP l (fun (x : A) _ => f x) = List.map f l.
+Proof.
+  remember (fun (x : A) _ => f x) as g.
+  funelim (map_InP l g) => //; simpl. f_equal. cbn in H.
+  now rewrite (H f0).
+Qed.
+
+Lemma In_size {A B} {x : A} {l : list A} (proj : A -> B) (size : B -> nat) : 
+  In x l -> size (proj x) < S (list_size (size ∘ proj) l).
+Proof.
+  induction l; cbn => //.
+  intros [->|hin]. lia. specialize (IHl hin); lia.
+Qed.
+
+Equations discr_construct (t : term) : Prop :=
+discr_construct (tConstruct ind n) := False ;
+discr_construct _ := True.
+
+Inductive construct_view : term -> Type :=
+| view_construct : forall ind n, construct_view (tConstruct ind n)
+| view_other : forall t, discr_construct t -> construct_view t.
+
+Equations construct_viewc t : construct_view t :=
+construct_viewc (tConstruct ind n) := view_construct ind n ;
+construct_viewc t := view_other t I.
+
+Section isEtaExp.
+  Context (Σ : global_context).
+  Definition lookup_minductive kn : option mutual_inductive_body :=
+    decl <- ETyping.lookup_env Σ kn;; 
+    match decl with
+    | ConstantDecl _ => None
+    | InductiveDecl mdecl => ret mdecl
+    end.
+
+  Definition lookup_inductive kn : option (mutual_inductive_body * one_inductive_body) :=
+    mdecl <- lookup_minductive (inductive_mind kn) ;;
+    idecl <- nth_error mdecl.(ind_bodies) (inductive_ind kn) ;;
+    ret (mdecl, idecl).
+  
+  Definition lookup_inductive_pars kn : option nat := 
+    mdecl <- lookup_minductive kn ;;
+    ret mdecl.(ind_npars).
+  
+  Definition lookup_constructor_pars_args kn c : option (nat * nat) := 
+    '(mdecl, idecl) <- lookup_inductive kn ;;
+    cdecl <- nth_error idecl.(ind_ctors) c ;;
+    ret (mdecl.(ind_npars), cdecl.2).
+    
+  Definition isEtaExp_app ind c k :=
+    match lookup_constructor_pars_args ind c with
+    | Some (npars, nargs) => leb (npars + nargs) k
+    | None => false
+    end.
+    
+  Import TermSpineView.
+
+  Equations? isEtaExp (e : EAst.term) : bool
+    by wf e (fun x y : EAst.term => size x < size y) :=
+  | e with TermSpineView.view e := {
+    | tRel i => true
+    | tEvar ev args => forallb_InP args (fun x H => isEtaExp x)
+    | tLambda na M => isEtaExp M
+    | tApp u v napp nnil with construct_viewc u := 
+      { | view_construct ind i => isEtaExp_app ind i (List.length v) && forallb_InP v (fun x H => isEtaExp x)
+        | view_other _ _ => isEtaExp u && forallb_InP v (fun x H => isEtaExp x) }
+    | tLetIn na b b' => isEtaExp b && isEtaExp b'
+    | tCase ind c brs => isEtaExp c && forallb_InP brs (fun x H => isEtaExp x.2)
+    | tProj p c => isEtaExp c
+    | tFix mfix idx => forallb_InP mfix (fun x H => isEtaExp x.(dbody))
+    | tCoFix mfix idx => forallb_InP mfix (fun x H => isEtaExp x.(dbody))
+    | tBox => true
+    | tVar _ => true
+    | tConst _ => true
+    | tConstruct ind i => isEtaExp_app ind i 0 }.
+  Proof.
+    all:try lia.
+    all:try apply (In_size); tea.
+    all:try lia.
+    - now apply (In_size id size). 
+    - rewrite size_mkApps.
+      change (fun x => size (id x)) with size in H. cbn.
+      now apply (In_size id size).
+    - now eapply size_mkApps_f.
+    - change (fun x => size (id x)) with size in H.
+      eapply (In_size id size) in H. unfold id in H.
+      change (fun x => size x) with size in H. 
+      pose proof (size_mkApps_l napp nnil). lia.
+    - eapply (In_size snd size) in H. cbn in H; lia.
+  Qed.
+  
+  Lemma isEtaExp_app_mon ind c i i' : i <= i' -> isEtaExp_app ind c i -> isEtaExp_app ind c i'.
+  Proof.
+    intros le.
+    unfold isEtaExp_app.
+    destruct lookup_constructor_pars_args as [[pars args]|]=> //.
+    do 2 elim: Nat.leb_spec => //. lia.
+  Qed.
+
+End isEtaExp.
+Global Hint Rewrite @forallb_InP_spec : isEtaExp.
+
+Opaque isEtaExp.
+
+Lemma In_All {A} {P : A -> Type} l : 
+(∀ x : A, In x l -> P x) -> All P l.
+Proof.
+induction l; cbn; constructor; auto.
+Qed.
+
+Ltac toAll := 
+repeat match goal with 
+  | [ H : forall x, In x ?l -> _ |- _ ] => eapply In_All in H
+end.
+
+Section something.
+
+Context (Σ : global_context).
+
+Hint Rewrite @forallb_InP_spec : isEtaExp.
+Transparent isEtaExp_unfold_clause_1.
+
+Lemma isEtaExp_mkApps_nonnil f v :
+  ~~ isApp f -> v <> [] ->
+  isEtaExp Σ (mkApps f v) = match construct_viewc f with 
+    | view_construct ind i => isEtaExp_app Σ ind i #|v| && forallb (isEtaExp Σ) v
+    | view_other t discr => isEtaExp Σ f && forallb (isEtaExp Σ) v
+  end.
+Proof.
+  rewrite isEtaExp_equation_1.
+  intros napp hv.
+  destruct (TermSpineView.view_mkApps (TermSpineView.view (mkApps f v)) napp hv) as [hna [hv' ->]].
+  cbn. destruct (construct_viewc f); cbn; simp isEtaExp => //.
+Qed.
+
+Lemma isEtaExp_mkApps f v : ~~ isApp f ->
+  isEtaExp Σ (mkApps f v) = match construct_viewc f with 
+    | view_construct ind i => isEtaExp_app Σ ind i #|v| && forallb (isEtaExp Σ) v
+    | view_other t discr => isEtaExp Σ f && forallb (isEtaExp Σ) v
+  end.
+Proof.
+  intros napp.
+  destruct v using rev_case; cbn.
+  - destruct construct_viewc; rewrite andb_true_r //.
+  - rewrite isEtaExp_mkApps_nonnil //. now destruct v; cbn; congruence.
+Qed.
+
+Lemma isEtaExp_Constructor ind i v :
+  isEtaExp Σ (mkApps (tConstruct ind i) v) = isEtaExp_app Σ ind i #|v| && forallb (isEtaExp Σ) v.
+Proof.
+  rewrite isEtaExp_mkApps //.
+Qed.
+
+Lemma isEtaExp_mkApps_intro t l : isEtaExp Σ t -> All (isEtaExp Σ) l -> isEtaExp Σ (mkApps t l).
+Proof.
+  revert t; induction l using rev_ind; auto.
+  intros t et a; eapply All_app in a as [].
+  depelim a0. clear a0.
+  destruct (decompose_app t) eqn:da.
+  rewrite (decompose_app_inv da) in et *.
+  pose proof (decompose_app_notApp _ _ _ da).
+  destruct l0. cbn.
+  - rewrite isEtaExp_mkApps //.
+    destruct construct_viewc. cbn. len.
+    rtoProp; repeat solve_all. cbn in et. simp isEtaExp in et.
+    eapply isEtaExp_app_mon; tea; lia.
+    eapply All_app_inv; eauto. rewrite et forallb_app /=.
+    rtoProp; repeat solve_all.
+  - rewrite isEtaExp_mkApps in et => //.
+    destruct construct_viewc.
+    rewrite -mkApps_app. rewrite isEtaExp_Constructor.
+    cbn. cbn. rtoProp; solve_all.
+    eapply isEtaExp_app_mon; tea. cbn. len. lia. now depelim H1.
+    depelim H1. solve_all. eapply All_app_inv => //.
+    eapply All_app_inv => //. eauto.
+    rewrite -mkApps_app. rewrite isEtaExp_mkApps //.
+    destruct (construct_viewc t0) => //.
+    move/andP: et => [] -> /=. rtoProp; solve_all.
+    rewrite forallb_app. rtoProp; repeat solve_all.
+    eapply All_app_inv; eauto.
+Qed.
+
+Lemma csubst_mkApps {a k f l} : csubst a k (mkApps f l) = mkApps (csubst a k f) (map (csubst a k) l).
+Proof.
+  induction l using rev_ind; simpl; auto.
+  rewrite mkApps_app /= IHl.
+  now rewrite -[EAst.tApp _ _](mkApps_app _ _ [_]) map_app.
+Qed.
+
+Lemma etaExp_csubst a k b : 
+  isEtaExp Σ a -> isEtaExp Σ b -> isEtaExp Σ (ECSubst.csubst a k b).
+Proof.
+  funelim (isEtaExp Σ b); cbn; simp isEtaExp; rewrite -?isEtaExp_equation_1; eauto;
+    toAll; repeat solve_all.
+  - intros. destruct Nat.compare => //.
+  - move/andP: H2 => [] etab etab'.
+    apply/andP. split; eauto.
+  - rtoProp. intuition eauto.
+    solve_all.
+  - move/andP: H1 => [] etaexp h.
+    rewrite csubst_mkApps /=.
+    rewrite isEtaExp_Constructor. solve_all.
+    rewrite map_length. rtoProp; solve_all. solve_all.
+  - rewrite csubst_mkApps /=.
+    move/andP: H2 => [] eu ev.
+    specialize (H _ k H1 eu).
+    eapply isEtaExp_mkApps_intro => //. solve_all.
+Qed.
+
+End something.
+
+Definition isEtaExp_constant_decl Σ cb := 
+  option_default (isEtaExp Σ) cb.(cst_body) true.
+
+Definition isEtaExp_decl Σ d :=
+  match d with
+  | ConstantDecl cb => isEtaExp_constant_decl Σ cb
+  | InductiveDecl idecl => true
+  end.
+
+Fixpoint isEtaExp_env (Σ : EAst.global_declarations) := 
+  match Σ with 
+  | [] => true
+  | decl :: Σ => isEtaExp_decl Σ decl.2 && isEtaExp_env Σ
+  end.
+
+(* Lemma strip_extends Σ Σ' : extends Σ Σ' ->
+  strip Σ t = strip Σ' t. *)
+
+Lemma isEtaExp_tApp Σ f u : isEtaExp Σ (mkApps f u) -> 
+  let (hd, args) := decompose_app (mkApps f u) in
+  match construct_viewc hd with
+  | view_construct kn c => isEtaExp_app Σ kn c #|args| && forallb (isEtaExp Σ) args
+  | view_other u discr => isEtaExp Σ hd && forallb (isEtaExp Σ) args
+  end.
+Proof.
+  destruct decompose_app eqn:da.
+  rewrite (decompose_app_inv da).
+  pose proof (decompose_app_notApp _ _ _ da).
+  destruct l. cbn -[isEtaExp].
+  intros eq; rewrite eq.
+  destruct (construct_viewc t) => //. simp isEtaExp in eq; now rewrite eq.
+  assert (t0 :: l <> []) by congruence.
+  revert da H0. generalize (t0 :: l). clear t0 l; intros l.
+  intros da nnil.
+  rewrite isEtaExp_mkApps //.
+Qed.
+
 From MetaCoq.Template Require Import config utils BasicAst Universes.
 From MetaCoq.Erasure Require Import EAst ETyping EAstUtils.
 
@@ -10,7 +320,7 @@ Local Unset Elimination Schemes.
 Inductive expanded : term -> Prop :=
 | expanded_tRel (n : nat) : expanded (tRel n)
 | expanded_tVar (id : ident) : expanded (tVar id)
-| expanded_tEvar (ev : nat) (args : list term) : expanded (tEvar ev args)
+| expanded_tEvar (ev : nat) (args : list term) : Forall expanded args -> expanded (tEvar ev args)
 | expanded_tLambda (na : name) (body : term) : expanded body -> expanded (tLambda na body)
 | expanded_tLetIn (na : name) (def : term)(body : term) : expanded def -> expanded body -> expanded (tLetIn na def body)
 | expanded_mkApps (f : term) (args : list term) : ~ isConstruct f -> expanded f -> Forall expanded args -> expanded (mkApps f args)
@@ -20,10 +330,10 @@ Inductive expanded : term -> Prop :=
 | expanded_tProj (proj : projection) (t : term) : expanded t -> expanded (tProj proj t)
 | expanded_tFix (mfix : mfixpoint term) (idx : nat) :  Forall (fun d => expanded d.(dbody)) mfix -> expanded (tFix mfix idx)
 | expanded_tCoFix (mfix : mfixpoint term) (idx : nat) : Forall (fun d => expanded d.(dbody)) mfix -> expanded (tCoFix mfix idx)
-| expanded_tPrim (prim : PCUICPrimitive.prim_val term) : expanded (tPrim prim)
 | expanded_tConstruct_app ind idx mind idecl cname c args :
     declared_constructor Σ (ind, idx) mind idecl (cname, c) ->
     #|args| >= ind_npars mind + c -> 
+    Forall expanded args ->
     expanded (mkApps (tConstruct ind idx) args)
 | expanded_tBox : expanded tBox.
 
@@ -33,7 +343,7 @@ Lemma expanded_ind :
 forall (Σ : global_declarations) (P : term -> Prop),
 (forall n : nat, P (tRel n)) ->
 (forall id : ident, P (tVar id)) ->
-(forall (ev : nat) (args : list term), P (tEvar ev args)) ->
+(forall (ev : nat) (args : list term), Forall (expanded Σ) args -> Forall P args -> P (tEvar ev args)) ->
 (forall (na : name) (body : term),
  expanded Σ body -> P body -> P (tLambda na body)) ->
 (forall (na : name) (def body : term),
@@ -41,13 +351,14 @@ forall (Σ : global_declarations) (P : term -> Prop),
  P def -> expanded Σ body -> P body -> P (tLetIn na def body)) ->
 (forall (f4 : term) (args : list term),
  ~ isConstruct f4 ->
- expanded Σ f4 -> P f4 -> Forall (expanded Σ) args -> P (mkApps f4 args)) ->
+ expanded Σ f4 -> P f4 -> Forall (expanded Σ) args -> Forall P args -> P (mkApps f4 args)) ->
 (forall c : kername, P (tConst c)) ->
 (forall (ind : inductive) (pars : nat) (discr : term)
    (branches : list (list name × term)),
  expanded Σ discr ->
  P discr ->
  Forall (fun br : list name × term => expanded Σ br.2) branches ->
+ Forall (fun br : list name × term => P br.2) branches ->
  P (tCase (ind, pars) discr branches)) ->
 (forall (proj : projection) (t : term),
  expanded Σ t -> P t -> P (tProj proj t)) ->
@@ -56,18 +367,91 @@ forall (Σ : global_declarations) (P : term -> Prop),
 (forall (mfix : mfixpoint term) (idx : nat),
  Forall (fun d : def term => expanded Σ (dbody d)) mfix ->  Forall (fun d : def term => P (dbody d)) mfix ->
  P (tCoFix mfix idx)) ->
-(forall prim, P (tPrim prim)) ->
 (forall (ind : inductive) (idx : nat) (mind : mutual_inductive_body)
    (idecl : one_inductive_body) (cname : ident) (c : nat) 
    (args : list term),
  declared_constructor Σ (ind, idx) mind idecl (cname, c) ->
- #|args| >= ind_npars mind + c -> P (mkApps (tConstruct ind idx) args)) ->
+ #|args| >= ind_npars mind + c -> Forall (expanded Σ) args -> Forall P args -> P (mkApps (tConstruct ind idx) args)) ->
 (P tBox) ->
 forall t : term, expanded Σ t -> P t.
 Proof. 
-  intros. revert t H13.
+  intros. revert t H12.
   fix f 2.
   intros t Hexp. destruct Hexp; eauto.
-  - eapply H8; eauto. induction H13; econstructor; cbn in *; eauto.
-  - eapply H9; eauto. induction H13; econstructor; cbn in *; eauto. 
+  - eapply H1; eauto. induction H12; econstructor; cbn in *; eauto.
+  - eapply H4; eauto. induction H13; econstructor; cbn in *; eauto.
+  - eapply H6; eauto. induction H12; econstructor; cbn in *; eauto.
+  - eapply H8; eauto. induction H12; econstructor; cbn in *; eauto.
+  - eapply H9; eauto. induction H12; econstructor; cbn in *; eauto.
+  - eapply H10; eauto. clear - H14 f. induction H14; econstructor; cbn in *; eauto.
+Qed.
+
+Local Hint Constructors expanded : core .
+Tactic Notation "simp_eta" "in" hyp(H) := simp isEtaExp in H; rewrite -?isEtaExp_equation_1 in H.
+Ltac simp_eta := simp isEtaExp; rewrite -?isEtaExp_equation_1.
+
+Lemma isEtaExp_app_expanded Σ ind idx n :
+   isEtaExp_app Σ ind idx n = true <->
+   exists mind idecl cname c,
+   declared_constructor Σ (ind, idx) mind idecl (cname, c) /\ n ≥ ind_npars mind + c.
+Proof.
+  unfold isEtaExp_app, lookup_constructor_pars_args, lookup_inductive, lookup_minductive.
+  split.
+  - intros H.
+    destruct lookup_env as [[| mind] | ] eqn:E; cbn in H; try congruence.
+    destruct nth_error as [ idecl | ] eqn:E2; cbn in H; try congruence.
+    destruct (nth_error (E.ind_ctors idecl) idx) as [ [cname ?] | ] eqn:E3; cbn in H; try congruence.
+    repeat esplit.
+    red. all: eauto. eapply leb_iff in H. lia.
+  - intros (? & ? & ? & ? & [[]] & Hle).
+    rewrite H. cbn. rewrite H0. cbn. rewrite H1. cbn.
+    eapply leb_iff. eauto.
+Qed.
+
+Lemma expanded_isEtaExp_app_ Σ ind idx n  mind idecl cname c :
+   declared_constructor Σ (ind, idx) mind idecl (cname, c) -> n ≥ ind_npars mind + c ->
+   isEtaExp_app Σ ind idx n = true.
+Proof.
+  intros. eapply isEtaExp_app_expanded. eauto 8.
+Qed.
+
+Lemma isEtaExp_expanded Σ t :
+  isEtaExp Σ t -> expanded Σ t.
+Proof.
+  funelim (isEtaExp Σ t); intros; solve_all; eauto.
+  - rewrite forallb_InP_spec in H0. eapply forallb_Forall in H0. eapply In_All in H.
+    econstructor. solve_all.
+  - eapply andb_true_iff in H1 as []; eauto.
+  - eapply isEtaExp_app_expanded in H as (? & ? & ? & ? & ? & ?).
+    eapply expanded_tConstruct_app with (args := []); eauto.
+  - eapply andb_true_iff in H1 as []. destruct ind. econstructor; eauto.
+    rewrite forallb_InP_spec in H2. eapply forallb_Forall in H2. 
+    eapply In_All in H0. solve_all.
+  - econstructor. rewrite forallb_InP_spec in H0. eapply forallb_Forall in H0. 
+    eapply In_All in H. solve_all.
+  - econstructor. rewrite forallb_InP_spec in H0. eapply forallb_Forall in H0. 
+    eapply In_All in H. solve_all.
+  - eapply andb_true_iff in H0 as []. eapply In_All in H.
+    rewrite forallb_InP_spec in H1. eapply forallb_Forall in H1.
+    eapply isEtaExp_app_expanded in H0 as (? & ? & ? & ? & ? & ?).
+    eapply expanded_tConstruct_app; eauto. solve_all.
+  - eapply andb_true_iff in H1 as []. rewrite forallb_InP_spec in H2. eapply forallb_Forall in H2.
+    econstructor.
+    + destruct u; inv Heq; eauto.
+    + eauto.
+    + eapply In_All in H0. solve_all.
+Qed.
+
+Lemma expanded_isEtaExp Σ t :
+  expanded Σ t -> isEtaExp Σ t.
+Proof.
+  induction 1; simp_eta; eauto.
+  all: try now (
+    (try (eapply andb_true_iff; split; eauto));
+    (try eapply forallb_Forall); 
+    eauto).
+  - eapply isEtaExp_mkApps_intro; eauto. solve_all.
+  - rewrite isEtaExp_Constructor. eapply andb_true_iff.
+    split. 2: eapply forallb_Forall.
+    2: solve_all. eapply expanded_isEtaExp_app_; eauto.
 Qed.
