pcuic/theories/TemplateToPCUICExpanded.v
@@ -13,7 +13,7 @@ Tactic Notation "wf_inv" ident(H) simple_intropattern(p) :=
 Local Hint Constructors expanded : expanded.
 
 Lemma trans_expanded {cf : checker_flags} {Σ} {wfΣ : Template.Typing.wf Σ} T :
-  let Σ' := trans_global_decls Σ in
+  let Σ' := trans_global_env Σ in
   WfAst.wf Σ T ->
   EtaExpand.expanded Σ T ->
   expanded Σ' (trans Σ' T).
@@ -22,6 +22,7 @@ Proof with eauto using expanded.
   induction exp; intros wf; cbn -[Σ']...
   all: try now (wf_inv wf []; eauto using expanded).
   all: try now (wf_inv wf [[]]; eauto using expanded).
+  - wf_inv wf ?. econstructor; eauto. solve_all.
   - wf_inv wf []. eapply expanded_mkApps with (args := [_]); cbn...
   - wf_inv wf [[[]]].
     forward IHexp; eauto.
@@ -30,7 +31,7 @@ Proof with eauto using expanded.
     destruct lookup_inductive as [[] | ]; cbn; eauto.
   - wf_inv wf []. eapply forall_decls_declared_constructor in H; eauto. 2: now eapply template_to_pcuic_env.
     eapply expanded_tConstruct_app with (args := []).
-    eauto. cbn. unfold trans_local. now rewrite context_assumptions_map.
+    eauto. cbn. unfold trans_local. now rewrite context_assumptions_map. econstructor.
   - wf_inv wf (mdecl' & idecl' & []). eapply forall_decls_declared_inductive in d; eauto. 2: now eapply template_to_pcuic_env.
     unfold Σ'.
     erewrite declared_inductive_lookup; eauto.
@@ -40,5 +41,5 @@ Proof with eauto using expanded.
   - wf_inv wf ?. econstructor. solve_all.
   - wf_inv wf ?. econstructor. solve_all.
   - wf_inv wf [[[]]]. eapply forall_decls_declared_constructor in H; eauto. 2: now eapply template_to_pcuic_env.
-    eapply expanded_tConstruct_app. eauto. cbn. unfold trans_local. now rewrite map_length context_assumptions_map.
+    eapply expanded_tConstruct_app. eauto. cbn. unfold trans_local. now rewrite map_length context_assumptions_map. solve_all.
 Qed.
